theories/iris_robust_examples.v
@@ -14,7 +14,7 @@ Unset Printing Implicit Defensive.
 Close Scope byte_scope.
 
 Notation "{{{ P }}} es {{{ v , Q }}}" :=
-  (∀ Φ, P -∗ (∀ v, Q -∗ Φ v) -∗ WP (es : iris.expr) @ NotStuck ; ⊤ {{ v, Φ v }}) (at level 50).
+  (□ ∀ Φ, P -∗ (∀ v, Q -∗ Φ v) -∗ WP (es : iris.expr) @ NotStuck ; ⊤ {{ v, Φ v }})%I (at level 50).
 
 Ltac take_drop_app_rewrite n :=
   match goal with
@@ -44,7 +44,7 @@ Section Examples.
 
   Import DummyHost.
 
-  Context `{!wfuncG Σ, !wtabG Σ, !wtabsizeG Σ, !wmemG Σ, !wmemsizeG Σ, !wglobG Σ, !wframeG Σ, !hvisG Σ, !hmsG Σ, !wtablimitG Σ, !wmemlimitG Σ,
+  Context `{!wfuncG Σ, !wtabG Σ, !wtabsizeG Σ, !wmemG Σ, !wmemsizeG Σ, !wglobG Σ, !wframeG Σ, !wtablimitG Σ, !wmemlimitG Σ,
         !logrel_na_invs Σ, HWP:host_program_logic}.
 
   Definition xx i := (VAL_int32 (Wasm_int.int_of_Z i32m i)).
@@ -89,48 +89,66 @@ Section Examples.
     WP e @ s; E {{ Φ }} -∗ (∀ v, Φ v -∗ Ψ v) -∗ WP e @ s; E {{ Ψ }}.
   Proof. iApply (wp_wand). Qed.
   
-  Definition lse a : iris.expr :=
-    to_e_list
+  Definition lse_expr a n :=
       [BI_const (xx 0);
        BI_const (xx 42);
-       BI_store T_i32 None 0%N 0%N] ++
-      [AI_invoke a] ++
-    to_e_list
-    [BI_const (xx 0);
-     BI_load T_i32 None 0%N 0%N].
+       BI_store T_i32 None 0%N 0%N;
+       BI_call a;
+       BI_const (xx 0);
+       BI_load T_i32 None 0%N 0%N;
+       BI_set_global n].
 
+  Definition lse a n :=
+    to_e_list (lse_expr a n).
 
-  Lemma lse_spec f n a C i es :
+  Lemma lse_spec f n j a C i es g k locs :
     (tc_label C) = [] ∧ (tc_return C) = None ->
+
     f.(f_inst).(inst_memory) !! 0 = Some n ->
-    be_typing (upd_local_label_return C [] [[]] (Some [])) es (Tf [] []) ->
+    f.(f_inst).(inst_funcs) !! j = Some a ->
+    f.(f_inst).(inst_globs) !! g = Some k ->
     
-    {{{ ↪[frame] f
+    be_typing (upd_local_label_return C locs [[]] (Some [])) es (Tf [] []) ->
+    
+    ⊢ {{{ ↪[frame] f
          ∗ na_own logrel_nais ⊤
-         ∗ na_inv logrel_nais (wfN (N.of_nat a)) ((N.of_nat a) ↦[wf] (FC_func_native i (Tf [] []) [] es))
+         ∗ na_inv logrel_nais (wfN (N.of_nat a)) ((N.of_nat a) ↦[wf] (FC_func_native i (Tf [] []) locs es))
          ∗ interp_instance (HWP:=HWP) C i
+         ∗ (∃ gv, N.of_nat k ↦[wg] {| g_mut := MUT_mut; g_val := gv |})
          ∗ ∃ c, (N.of_nat n) ↦[wms][ 0%N ] (bits (VAL_int32 c)) }}}
-      lse a
-      {{{ w, (⌜w = trapV⌝ ∨ ⌜w = immV [xx 42]⌝
+      lse j g
+      {{{ w, (⌜w = trapV⌝ ∨ (⌜w = immV []⌝
+                                      ∗ (N.of_nat k) ↦[wg] {| g_mut := MUT_mut; g_val := xx 42 |}
                                       ∗ (N.of_nat n) ↦[wms][ 0%N ] (bits (xx 42))
-                                      ∗ na_own logrel_nais ⊤)
+                                      ∗ na_own logrel_nais ⊤))
                ∗ ↪[frame] f }}}.
   Proof.
-    iIntros (Hc Hn Hes Φ) "(Hf & Hown & #Ha & #Hi & Hn) HΦ".
+    iIntros (Hc Hn Ha Hg Hes Φ). iModIntro.
+    iIntros "(Hf & Hown & #Ha & #Hi & Hg & Hn) HΦ".
     iDestruct "Hn" as (c) "Hn".
+    iDestruct "Hg" as (gv) "Hg".
     iApply (wp_wand with "[-HΦ] HΦ").
 
-    unfold lse. simpl.
+    unfold lse.
 
     take_drop_app_rewrite 3.
     iApply (wp_seq _ _ _ (λ w, (⌜w = immV []⌝ ∗ N.of_nat n↦[wms][0] bits (xx 42)) ∗ ↪[frame] f)%I).
     iSplitR;[by iIntros "[[%Hcontr _] _]"|].
-    iSplitR "Hown".
+    iSplitR "Hown Hg".
     { unfold serialise_i32. simpl. iApply (wp_store (λ w, ⌜w = immV ([])⌝)%I with "[$Hf Hn]");eauto.
       by rewrite Memdata.encode_int_length. }
     iIntros (w) "[[-> Hn] Hf]". iSimpl.
 
-    take_drop_app_rewrite_twice 0 2.
+    take_drop_app_rewrite_twice 0 3.
+    iApply wp_wasm_empty_ctx.
+    iApply wp_base_push;auto.
+    iApply (wp_call_ctx with "Hf");eauto.
+    iNext. iIntros "Hf".
+    iApply wp_base_pull.
+    iApply wp_wasm_empty_ctx.
+    iSimpl.
+    
+    take_drop_app_rewrite_twice 0 3.
     iApply wp_wasm_empty_ctx.
     iApply wp_base_push;auto.
     rewrite -(app_nil_r [_]).
@@ -156,9 +174,9 @@ Section Examples.
       iMod ("Hcls" with "[$]") as "Hown". iModIntro.
       simpl.
 
-      iDestruct (be_fundamental_local _ _ [] _ [] with "Hi") as "Hl";eauto.
-      iSpecialize ("Hl" $! _ [] with "Hf Hown []").
-      { iRight. iExists _. iSplit;eauto. }
+      iDestruct (be_fundamental_local _ _ [] _ locs with "Hi") as "Hl";eauto.
+      iSpecialize ("Hl" $! _ (n_zeros locs) with "Hf Hown []").
+      { iRight. iExists _. iSplit;eauto. rewrite app_nil_l. iApply n_zeros_interp_values. }
       unfold interp_expression_closure. simpl.
       iApply (wp_wand with "Hl").
       iIntros (v) "[[[H|H] Hown] HH]";iFrame. iRight;auto.
@@ -170,11 +188,303 @@ Section Examples.
     iDestruct (big_sepL2_length with "Heq") as %Heq. destruct ws;[|done].
     iSimpl.
 
-    iApply (wp_wand _ _ _ (λ vs, (⌜vs = immV _⌝ ∗ _) ∗ _)%I with "[Hn Hf]").
+    take_drop_app_rewrite 2.
+    iApply (wp_seq _ _ _ (λ v, (⌜v = immV _⌝ ∗ _) ∗ _)%I).
+    iSplitR;[by iIntros "[[% _] _]";done|].
+    iSplitL "Hn Hf".
     { iApply wp_load;eauto;[|iFrame];eauto. }
+    iIntros (v) "[[-> Hn] Hf]". iSimpl.
 
-    iIntros (v) "[[-> Hn] Hf]". iFrame.
+    iApply (wp_wand _ _ _ (λ v, (⌜v = immV _⌝ ∗ _) ∗ _)%I with "[Hf Hg]").
+    { iApply (wp_set_global with "[] Hf Hg"); eauto. }
+
+    iIntros (v) "[[-> Hg] Hf]". iFrame.
     iRight. iFrame. auto.
   Qed.
 
 End Examples.
+
+Section Examples_host.
+
+  Import DummyHost.
+
+  Context `{!wfuncG Σ, !wtabG Σ, !wtabsizeG Σ, !wmemG Σ, !wmemsizeG Σ, !wglobG Σ, !wframeG Σ, !hvisG Σ, !hmsG Σ, !wtablimitG Σ, !wmemlimitG Σ,
+        !logrel_na_invs Σ, HWP:host_program_logic,!hvisG Σ, !hmsG Σ}.
+
+
+  Notation "{{{ P }}} es {{{ v , Q }}}" :=
+    (□ ∀ Φ, P -∗ (∀ v, Q -∗ Φ v) -∗ WP (es : host_expr) @ NotStuck ; ⊤ {{ v, Φ v }})%I (at level 50).
+
+  Notation " n ↪[vis]{ q } v" := (ghost_map_elem (V := module_export) visGName n q v%V)
+                           (at level 20, q at level 5, format " n ↪[vis]{ q } v") .
+  Notation " n ↪[vis] v" := (ghost_map_elem (V := module_export) visGName n (DfracOwn 1) v%V)
+                          (at level 20, format " n ↪[vis] v").
+  
+  Notation " n ↪[mods]{ q } v" := (ghost_map_elem (V := module) msGName n q v%V)
+                           (at level 20, q at level 5, format " n ↪[mods]{ q } v") .
+  Notation " n ↪[mods] v" := (ghost_map_elem (V := module) msGName n (DfracOwn 1) v%V)
+                               (at level 20, format " n ↪[mods] v").
+
+  Lemma wp_wand_host s E (e : host_expr) (Φ Ψ : host_val -> iProp Σ) :
+    WP e @ s; E {{ Φ }} -∗ (∀ v, Φ v -∗ Ψ v) -∗ WP e @ s; E {{ Ψ }}.
+  Proof. iApply (weakestpre.wp_wand). Qed.
+  
+
+  Definition lse_module :=
+    {| mod_types := [Tf [] []; Tf [] []];
+       mod_funcs :=  [ {|
+          modfunc_type := Mk_typeidx 0 ;
+          modfunc_locals := [] ;
+          modfunc_body := lse_expr 0 0
+        |} ] ;
+      mod_tables := [];
+      mod_mems := [ {| lim_min := 4%N ; lim_max := None |} ];
+      mod_globals := (* [ {| modglob_type := {| tg_mut := MUT_mut; tg_t := T_i32 |} ; modglob_init := [BI_const (xx 0)] |} ]; *) [];
+      mod_elem := [];
+      mod_data := [];
+      mod_start := Some {| modstart_func := Mk_funcidx 1 |};
+      mod_imports := [ {| imp_module := list_byte_of_string "Adv";
+                         imp_name := list_byte_of_string "adv_call";
+                         imp_desc := ID_func 0 |};
+                       {| imp_module := list_byte_of_string "Ret";
+                         imp_name := list_byte_of_string "ret_glob";
+                         imp_desc := ID_global {| tg_mut := MUT_mut; tg_t := T_i32 |} |} ];
+      mod_exports := []
+    |}.
+
+  Definition lse_func_impts : seq.seq extern_t := [ET_func (Tf [] [])].
+  Definition lse_glob_impts : seq.seq extern_t := [ET_glob {| tg_mut := MUT_mut; tg_t := T_i32 |} ].
+
+  Ltac type_next :=
+  match goal with
+  | |- context [ be_typing _ ?e _  ] =>
+      rewrite -(list.take_drop (length e - 1) e);simpl take; simpl drop;
+      eapply bet_composition;[|econstructor;eauto];simpl
+  end.
+  
+  Lemma lse_module_typing :
+    module_typing lse_module (lse_func_impts ++ lse_glob_impts) [].
+  Proof.
+    exists [Tf [] []],[ (* {| tg_mut := MUT_mut; tg_t := T_i32 |} *)]. simpl.
+    repeat split;eauto.
+    { apply Forall2_cons. split;auto. cbn.
+      repeat split;auto.
+      repeat type_next.
+      rewrite <- (take_drop 1 [BI_const _;_]);simpl take;simpl drop.
+      eapply bet_composition;[econstructor|].
+      rewrite <- (app_nil_r [typeof _]);simpl typeof.
+      rewrite <- (take_drop 1 [T_i32;_]);simpl take;simpl drop.
+      eapply bet_weakening. apply bet_const. }
+    { apply Forall2_cons. split;auto.
+      apply Forall2_cons. split;auto. }
+  Qed.
+
+  Definition adv_lse_instantiate :=
+    [ ID_instantiate [0%N] 0 [] ;
+      ID_instantiate [] 1 [0%N;1%N] ].
+
+  
+  Lemma instantiate_lse adv_module g_ret wret :
+    module_typing adv_module [] lse_func_impts -> (* we assume the adversary module has an export of the () → () *)
+    mod_start adv_module = None -> (* that it does not have a start function *)
+    module_restrictions adv_module -> (* that it adheres to the module restrictions (i.e. only constant initializers for globals) *)
+    typeof wret = T_i32 -> (* the imported return global has type i32 *)
+
+    ⊢ {{{ g_ret ↦[wg] {| g_mut := MUT_mut; g_val := wret |} ∗
+          0%N ↪[mods] adv_module ∗
+          1%N ↪[mods] lse_module ∗
+          na_own logrel_nais ⊤ ∗
+          (∃ name, 1%N ↪[vis] {| modexp_name := name; modexp_desc := MED_global (Mk_globalidx (N.to_nat g_ret)) |}) ∗
+          (∃ vs, 0%N ↪[vis] vs) }}}
+        ((adv_lse_instantiate,[]) : host_expr)
+      {{{ v, ⌜v = (trapV : host_val)⌝ ∨ g_ret ↦[wg] {| g_mut := MUT_mut; g_val := xx 42|} }}} .
+  Proof.
+    iIntros (Htyp Hnostart Hrestrict Hgrettyp).
+    iModIntro. iIntros (Φ) "(Hgret & Hmod_adv & Hmod_lse & Hown & Hvis1 & Hvis) HΦ".
+    iApply (wp_seq_host_nostart with "[$Hmod_adv] [Hvis] ") => //.
+    { iIntros "Hmod_adv".
+      iApply weakestpre.wp_mono.
+      2: iApply (instantiation_spec_operational_no_start _ _ _ [] [] _ _ _ _ ∅ ∅ ∅ ∅);eauto;iFrame.
+      2: cbn; repeat iSplit =>//.
+      iIntros (v) "[$ Hv']". iExact "Hv'". }
+
+    iIntros (w) "(_ & _ & Hinst_adv) Hmod_adv".
+    iDestruct "Hinst_adv" as (inst_adv g_adv_inits (?&?&?&?&?&?) Htyp_inits) "(Hinst_adv_res & Hadv_exports)".
+    iDestruct (big_sepL2_length with "Hadv_exports") as %Hexp_len.
+    destruct (mod_exports adv_module) eqn:Hexp;[done|].
+    destruct l;[|done].
+    iDestruct "Hadv_exports" as "[Hn _]".
+    revert Htyp. rewrite module_typing_body_eq =>Htyp.
+    destruct Htyp as [fts [gts Htyp]].
+    assert (Hmod:=Htyp).
+    remember adv_module as advm.
+    destruct adv_module. rewrite Heqadvm in Hexp.
+    rewrite Heqadvm in Hmod.
+    
+    simpl in Hexp. subst mod_exports.
+    destruct Hmod as (Hmod&_&_&_&_&_&_&Himpts&Hexpts).
+    apply Forall2_length in Himpts. destruct mod_imports;[|done].
+    unfold lse_func_impts in Hexpts. simpl in Hexpts.
+    apply Forall2_cons in Hexpts as [He _].
+    unfold module_export_typing in He. simpl in He.
+    destruct (modexp_desc m) eqn:Hm;[destruct f|by destruct t|by destruct m0|by destruct g].
+    apply andb_true_iff in He as [Hle He].
+    destruct (nth_error fts n) eqn:Hn;[|done].
+    revert He. move/eqP=>He. subst f.
+    iDestruct "Hn" as (name) "Hn".
+
+    rewrite Heqadvm.
+    iDestruct "Hinst_adv_res" as "(Hresf & Hrest & Hresm & Hresg) /=".
+    rewrite /get_import_func_count
+            /get_import_mem_count
+            /get_import_table_count
+            /get_import_global_count /=.
+    rewrite !drop_0 -Heqadvm.
+    rewrite nth_error_lookup in Hn.
+    eapply Forall2_lookup_r in Hmod as [mf [Hmf Htypf]];[|eauto].
+    destruct mf. simpl in Htypf.
+    destruct modfunc_type. destruct Htypf as (Hlef & Hnthf & Htypf).
+    revert Hlef. move/ssrnat.leP=>Hlef.
+    assert (n0 < length mod_types) as Hlt;[lia|].
+    rewrite Heqadvm /= in H.
+    apply lookup_lt_is_Some in Hlt as [t Ht].
+    rewrite - nth_error_lookup in Ht.
+    erewrite nth_error_nth in Hnthf;eauto.
+    revert Hnthf;move/eqP=>heq. subst t.
+    iDestruct (big_sepL2_length with "Hresf") as %Hinstf_len.
+    apply lookup_lt_Some in Hmf as Hlt'.
+    rewrite Hinstf_len in Hlt'.
+    apply lookup_lt_is_Some in Hlt' as [advf Hadv].
+    iDestruct (big_sepL2_lookup_acc with "Hresf") as "[Hadvf Hcls]";[eauto..|].
+    simpl.
+    rewrite - nth_error_lookup in Hadv.
+    rewrite H.
+    erewrite !nth_error_nth;eauto.
+    
+    iDestruct "Hvis1" as (gr) "Hvis1".
+
+    iApply (wp_wand_host _ _ _ (λ v, _ ∗ ↪[frame]empty_frame)%I with "[-HΦ] [HΦ]");cycle 1.
+    { iIntros (v) "[Hv ?]". iApply "HΦ". iExact "Hv". }
+    { iApply (instantiation_spec_operational_start with "[$Hmod_lse Hadvf Hgret Hn Hvis1]");[eauto|..].
+      { apply lse_module_typing. }
+      { unfold import_resources_host.
+        instantiate (5:=[_;_]). iFrame "Hn Hvis1".
+        unfold import_resources_wasm_typecheck,export_ownership_host.
+        iSimpl. do 3 iSplit =>//.
+        { instantiate (1:={[N.to_nat g_ret := {| g_mut := MUT_mut; g_val := wret |} ]}).
+          instantiate (1:=∅).
+          instantiate (1:=∅).
+          instantiate (1:= {[advf := (FC_func_native inst_adv (Tf [] []) modfunc_locals modfunc_body)]}).
+          iPureIntro. cbn. repeat split;auto.
+          all: rewrite dom_singleton_L;clear;set_solver.
+        }
+        { iSplitR "Hgret".
+          { iExists _. iFrame. repeat iSplit;auto.
+            iPureIntro. apply lookup_singleton. }
+          { iSplit =>//. iExists _,_. rewrite N2Nat.id. iFrame. repeat iSplit;auto.
+            iPureIntro. apply lookup_singleton.
+            iPureIntro. cbn. rewrite Hgrettyp. done. }
+        }
+      }
+      { iIntros (idnstart) "Hf Hr".
+        iDestruct "Hr" as "(Hmod_lse & [Himph _] & [%Hdom [Himpr [Hgret _]]] & H)".
+        iSimpl in "Himpr Hgret".
+        iDestruct "Himpr" as (cl) "[Hcl %Hcl]". destruct Hcl as [Hlookcl Hcltyp].
+        rewrite lookup_singleton in Hlookcl. inversion Hcltyp;inversion Hlookcl.
+        iDestruct ("Hcls" with "Hcl") as "Hresf".
+        iDestruct "Hgret" as (g gt) "(Hgret & %Hlookg & %Hgteq & %Hagree)".
+        rewrite lookup_singleton in Hlookg. inversion Hgteq;inversion Hlookg. rewrite N2Nat.id.
+        
+        iApply weakestpre.fupd_wp.
+        iMod (interp_instance_alloc with "[] [] [] [] [Hrest Hresm Hresg Hresf]") as "[#Hi [#Hires _]]";
+          [apply Htyp|repeat split;eauto|eauto|..].
+        2,3,4: by instantiate (1:=∅).
+        { rewrite Heqadvm /=. auto. }
+        { instantiate (1:=∅). iSplit;auto. }
+        { rewrite /module_inst_resources_wasm Heqadvm /=
+                  /get_import_table_count
+                  /get_import_mem_count
+                  /get_import_global_count
+                  /get_import_func_count /= !drop_0 -H.
+          iFrame. }
+
+        rewrite !app_nil_l.
+        iDestruct (big_sepL2_lookup with "Hires") as "Ha".
+        { rewrite Heqadvm /=. eauto. }
+        { rewrite Heqadvm /= /get_import_func_count /= drop_0 /= -nth_error_lookup. eauto. }
+        iSimpl in "Ha". erewrite H, nth_error_nth;eauto.
+
+        iApply wp_host_wasm;[apply HWEV_invoke|]. iSimpl in "H".
+        iDestruct "H" as (inst g_inits Hinst Hg_inits) "[Hlse _]".
+        destruct g_inits;[|done].
+        cbn in Hinst. destruct Hinst as (Hinst_typ & Hinst_f & _ & _ & Hinst_g & Hstart).
+        destruct (inst_funcs inst) eqn:Hinstfuncseq;[done|].
+        destruct l;[done|]. simpl in Hstart. revert Hstart. move/eqP =>Hstart. subst f0.
+        destruct (inst_globs inst) eqn:Hinstglobseq;[by inversion Hinst_g|].
+        simpl in Hinst_f, Hinst_g.
+        apply prefix_cons_inv_1 in Hinst_f as Heq.
+        apply prefix_cons_inv_1 in Hinst_g as Heq'. subst f g0.
+        
+        iDestruct "Hlse" as "[Hlsef [_ [Hlsem _]]]". iClear "Hmod_lse".
+        
+        rewrite /lse_module /get_import_func_count /get_import_mem_count /get_import_global_count !drop_0.
+        iSimpl in "Hlsef Hlsem".
+        rewrite Hinstfuncseq. iSimpl in "Hlsef".
+        iDestruct "Hlsef" as "[Hidnstart _]".
+        rewrite Hinst_typ. iSimpl in "Hidnstart".
+        clear Hdom.
+        iDestruct (big_sepL2_length with "Hlsem") as %Hinstmem_len.
+        simpl in Hinstmem_len.
+        destruct (inst_memory inst) eqn:Hinstmemeq;[done|].
+        iDestruct "Hlsem" as "[Hm _]".
+        
+        take_drop_app_rewrite 0.
+        iApply (wp_invoke_native with "Hf Hidnstart");[eauto|eauto..|].
+        iModIntro. iNext. iIntros "[Hf Hidnstart]".
+        iApply (wp_frame_bind with "Hf"). iIntros "Hf".
+        take_drop_app_rewrite 0. iApply (wp_block with "Hf");[auto..|].
+        iNext. iIntros "Hf".
+        iApply wp_wasm_empty_ctx.
+        iApply wp_label_push_nil.
+        iApply wp_ctx_bind;[simpl;auto|]. repeat erewrite app_nil_l.
+
+        iApply (wp_wand with "[Hf Hgret Hm Hown]").
+        { iApply (lse_spec with "[$Hi $Hf $Hown $Ha Hgret Hm]");[by simpl|simpl..|].
+          { rewrite Hinstmemeq;eauto. }
+          { rewrite Hinstfuncseq;eauto. }
+          { rewrite Hinstglobseq;eauto. }
+          { unfold upd_local_label_return;simpl.
+            rewrite Heqadvm /=. eauto. }
+          { iSplitR "Hm". rewrite N2Nat.id. eauto.
+            iDestruct "Hm" as "[Hm _]". iSimpl in "Hm".
+            iDestruct "Hm" as "(Hm1 & Hm2 & Hm3 & Hm4 & _)". 
+            iExists (Wasm_int.int_of_Z i32m 0).
+            unfold serialise_i32. cbn. iFrame. done. }
+          iIntros (w0) "Hw". iExact "Hw".
+        }
+
+        iIntros (wres) "[[-> | [-> [Hgret Hm]]] Hf]". 
+        { iApply (wp_wand_ctx with "[Hf]").
+          { take_drop_app_rewrite_twice 0 0. iApply (wp_trap_ctx with "Hf");auto. }
+          iIntros (v) "[-> Hf]".
+          iExists _. iFrame "Hf".
+          iIntros "Hf".
+          iApply (wp_frame_trap with "Hf").
+          iNext. by iLeft. }
+
+        rewrite N2Nat.id. simpl of_val.
+
+        iApply (wp_wand_ctx _ _ _ (λ v, ⌜v = immV []⌝ ∗ _)%I with "[Hf]").
+        { iApply (wp_val_return with "Hf");auto.
+          iIntros "Hf". iApply wp_value;eauto. done. }
+        iIntros (v) "[-> Hf]".
+        iExists _. iFrame "Hf".
+        iIntros "Hf".
+        iApply (wp_frame_value with "Hf");eauto.
+      }
+    }
+    Unshelve. apply HWP.
+  Qed.
+  
+
+End Examples_host.
